\section*{附录 A.}\label{sec:appendix_a}
\addcontentsline{toc}{section}{附录 A.}

在这个附录中，我们推导出本文公式（6）中给出的熵的表达式。

\begin{equation*}
    \begin{aligned}
S(\sigma_{\text{max}}) =
& - \sum_{i=0}^{ng} p_{i_R} \ln p_{i_R} - \sum_{i=0}^{ng} p_{i_{\overline{R}}} \ln p_{i_{\overline{R}}}
\\
\text{with } & p_{i_R} = \frac{H_R[i]}{\text{Card}\{R(\sigma_{\text{max}})\}} \text{ and } p_{i_{\overline{R}}} = \frac{H_{\overline{R}}[i]}{\text{Card}\{\overline{R}(\sigma_{\text{max}})\}}
\\
\text{with } & H_R \text{ and } H_{\overline{R}} \text{ histograms of } R(\sigma_{\text{max}}) \text{ and } \overline{R}(\sigma_{\text{max}})
\\
S(\sigma_{\text{max}}) =
& - \frac{1}{\text{Card}\{R(\sigma_{\text{max}})\}} \sum_{i=0}^{ng}H_R[i]\ln(H_R[i])
- \frac{1}{\text{Card}\{\overline{R}(\sigma_{\text{max}})\}} \sum_{i=0}^{ng}H_{\overline{R}}[i]\ln(H_{\overline{R}}[i])
\\
& + \frac{1}{\text{Card}\{R(\sigma_{\text{max}})\}} \sum_{i=0}^{ng}H_R[i]\ln(\text{Card}\{R(\sigma_{\text{max}})\})
+ \frac{1}{\text{Card}\{\overline{R}(\sigma_{\text{max}})\}} \sum_{i=0}^{ng}H_{\overline{R}}[i]\ln(\text{Card}\{\overline{R}(\sigma_{\text{max}})\})
\\
S(\sigma_{\text{max}}) =
& - \frac{1}{\text{Card}\{R(\sigma_{\text{max}})\}} \sum_{i=0}^{ng}H_R[i]\ln(H_R[i])
- \frac{1}{\text{Card}\{\overline{R}(\sigma_{\text{max}})\}} \sum_{i=0}^{ng}H_{\overline{R}}[i]\ln(H_{\overline{R}}[i])
\\
& + \ln(\text{Card}\{R(\sigma_{\text{max}})\}) + \ln(\text{Card}\{\overline{R}(\sigma_{\text{max}})\})
\\
S(\sigma_{\text{max}}) =
& - \frac{1}{\text{Card}\{R(\sigma_{\text{max}})\}} \sum_{i=0}^{ng}H_R[i]\ln(H_R[i])
- \frac{1}{\text{Card}\{\overline{R}(\sigma_{\text{max}})\}} \sum_{i=0}^{ng}H_{\overline{R}}[i]\ln(H_{\overline{R}}[i])
\\
& + \ln(\text{Card}\{R(\sigma_{\text{max}})\} \cdot \text{Card}\{\overline{R}(\sigma_{\text{max}})\})
.
    \end{aligned}
\end{equation*}

%    \, \text{with} \, H_R \, and \, H_{\overline{R}} \, \text{histograms of} \, R(\sigma_{\text{max}}) \, \text{and} \, \overline{R}(\sigma_{\text{max}}).